Various trivial tweaks to asmScript.

targets/asmScript.sml
@@ -1,8 +1,11 @@
-open HolKernel Parse boolLib bossLib wordsTheory;
+open HolKernel Parse boolLib bossLib
+open wordsTheory;
 
-val _ = new_theory "asm";
+val () = new_theory "asm"
 
-(* This script defines the syntax and semantics of a small general-
+(* -------------------------------------------------------------------------
+
+   This script defines the syntax and semantics of a small general-
    purpose assembly language (without labels).
 
    The intention is that each instruction in this assembly language
@@ -64,106 +67,106 @@ val _ = new_theory "asm";
    non-deterministic behaviour. It is up to the target provider to
    prove that the supplied encode function provides deterministic
    behaviour in the assembly language, i.e. instruction encodings only
-   overlap if the assembly semantics also matches precisely. *)
+   overlap if the assembly semantics also matches precisely.
+
+   ------------------------------------------------------------------------- *)
 
 (* -- syntax of ASM instruction -- *)
 
-val _ = temp_type_abbrev("reg",``:num``);
-val _ = temp_type_abbrev("imm",``:'a word``);
+val () = Parse.temp_type_abbrev ("reg", ``:num``)
+val () = Parse.temp_type_abbrev ("imm", ``:'a word``)
 
-val _ = Datatype `
-  reg_imm = Reg reg | Imm ('a imm) `
+val () = Datatype `
+  reg_imm = Reg reg | Imm ('a imm)`
 
-val _ = Datatype `
-  binop = Add | Sub | And | Or | Xor `
+val () = Datatype `
+  binop = Add | Sub | And | Or | Xor`
 
-val _ = Datatype `
-  cmp = Equal | Lower | Less | Test `
+val () = Datatype `
+  cmp = Equal | Lower | Less | Test`
 
-val _ = Datatype `
-  shift = Lsl | Lsr | Asr `
+val () = Datatype `
+  shift = Lsl | Lsr | Asr`
 
-val _ = Datatype `
+val () = Datatype `
   arith = Binop binop reg reg ('a reg_imm)
-        | Shift shift reg reg num `
+        | Shift shift reg reg num`
 
-val _ = Datatype `
-  addr = Addr reg ('a word) `
+val () = Datatype `
+  addr = Addr reg ('a word)`
 
-val _ = Datatype `
-  mem_op = Load | Load8 | Load32
-         | Store | Store8 | Store32 `
+val () = Datatype `
+  mem_op = Load  | Load8  | Load32
+         | Store | Store8 | Store32`
 
-val _ = Datatype `
+val () = Datatype `
   inst = Const reg ('a word)
        | Arith ('a arith)
-       | Mem mem_op reg ('a addr) `
+       | Mem mem_op reg ('a addr)`
 
-val _ = Datatype `
+val () = Datatype `
   asm = Skip
       | Inst ('a inst)
-      | Jump ('a word) (('a inst) option) (* delay slot *)
-      | JumpCmp cmp reg ('a reg_imm) ('a word) (('a inst) option)
+      | Jump ('a word) ('a inst option) (* delay slot *)
+      | JumpCmp cmp reg ('a reg_imm) ('a word) ('a inst option)
       | Call ('a word) reg
       | JumpReg reg
-      | Loc reg ('a word) `
+      | Loc reg ('a word)`
 
 (* -- ASM target-specific configuration -- *)
 
-val _ = Datatype `
+val () = Datatype `
   asm_config =
-    <| ISA_name : string
-     ; reg_count : num
-     ; avoid_regs : num list
-     ; link_reg : num
-     ; allow_call : bool
-     ; has_delay_slot : bool
-     ; two_reg_arith : bool
-     ; imm_min : 'a word
-     ; imm_max : 'a word
+    <| ISA_name        : string
+     ; reg_count       : num
+     ; avoid_regs      : num set
+     ; link_reg        : num
+     ; allow_call      : bool
+     ; has_delay_slot  : bool
+     ; two_reg_arith   : bool
+     ; imm_min         : 'a word
+     ; imm_max         : 'a word
      ; addr_offset_min : 'a word
      ; addr_offset_max : 'a word
      ; jump_offset_min : 'a word
      ; jump_offset_max : 'a word
-     ; code_alignment : num
-     |> `
+     ; code_alignment  : num
+     |>`
 
 val reg_ok_def = Define `
-  reg_ok r c = r < c.reg_count /\ ~(MEM r c.avoid_regs)`;
+  reg_ok r c = r < c.reg_count /\ r NOTIN c.avoid_regs`
 
 val imm_ok_def = Define `
-  imm_ok w c = c.imm_min < w /\ w < c.imm_max`;
+  imm_ok w c = c.imm_min <= w /\ w <= c.imm_max`
 
 val reg_imm_ok_def = Define `
   (reg_imm_ok (Reg r) c = reg_ok r c) /\
-  (reg_imm_ok (Imm w) c = imm_ok w c)`;
+  (reg_imm_ok (Imm w) c = imm_ok w c)`
 
 val arith_ok_def = Define `
   (arith_ok (Binop b r1 r2 ri) c =
      (c.two_reg_arith ==> (r1 = r2)) /\
      reg_ok r1 c /\ reg_ok r2 c /\ reg_imm_ok ri c) /\
   (arith_ok (Shift l r1 r2 n) c =
-     reg_ok r1 c /\ reg_ok r2 c)`;
+     reg_ok r1 c /\ reg_ok r2 c)`
 
 val cmp_ok_def = Define `
-  cmp_ok (cmp:cmp) r ri c <=>
-     reg_ok r c /\ reg_imm_ok ri c`;
+  cmp_ok (cmp: cmp) r ri c = reg_ok r c /\ reg_imm_ok ri c`
 
 val addr_offset_ok_def = Define `
-  addr_offset_ok w c = c.addr_offset_min < w /\ w < c.addr_offset_max`;
+  addr_offset_ok w c = c.addr_offset_min <= w /\ w <= c.addr_offset_max`
 
 val jump_offset_ok_def = Define `
-  jump_offset_ok w c = c.jump_offset_min < w /\ w < c.jump_offset_max /\
-                       (w2n w MOD c.code_alignment = 0)`;
+  jump_offset_ok w c = c.jump_offset_min <= w /\ w <= c.jump_offset_max /\
+                       (w2n w MOD c.code_alignment = 0)`
 
 val addr_ok_def = Define `
-  addr_ok (Addr r w) c =
-    reg_ok r c /\ addr_offset_ok w c`;
+  addr_ok (Addr r w) c = reg_ok r c /\ addr_offset_ok w c`
 
 val inst_ok_def = Define `
   (inst_ok (Const r w) c = reg_ok r c) /\
   (inst_ok (Arith x) c = arith_ok x c) /\
-  (inst_ok (Mem m r a) c = reg_ok r c /\ addr_ok a c)`;
+  (inst_ok (Mem m r a) c = reg_ok r c /\ addr_ok a c)`
 
 val asm_ok_def = Define `
   (asm_ok (Skip) c = T) /\
@@ -176,57 +179,52 @@ val asm_ok_def = Define `
      jump_offset_ok w c /\ cmp_ok cmp r ri c /\
      case i of NONE => ~c.has_delay_slot
              | SOME x => inst_ok x c /\ c.has_delay_slot) /\
-  (asm_ok (Call w r) c = reg_ok r c /\ c.allow_call /\
-                         (c.link_reg = r) /\ jump_offset_ok w c) /\
+  (asm_ok (Call w r) c =
+     reg_ok r c /\ c.allow_call /\
+     (c.link_reg = r) /\ jump_offset_ok w c) /\
   (asm_ok (JumpReg r) c = reg_ok r c) /\
-  (asm_ok (Loc r w) c = reg_ok r c /\ jump_offset_ok w c)`;
+  (asm_ok (Loc r w) c = reg_ok r c /\ jump_offset_ok w c)`
 
 (* -- semantics of ASM program -- *)
 
-val _ = Datatype `
+val () = Datatype `
   asm_state =
-    <| regs : num -> 'a word
-     ; mem : 'a word -> word8
+    <| regs       : num -> 'a word
+     ; mem        : 'a word -> word8
      ; mem_domain : 'a word set
-     ; pc : 'a word
-     ; failed : bool
-     |> `
+     ; pc         : 'a word
+     ; failed     : bool
+     |>`
 
-val upd_pc_def   = Define `upd_pc pc s = s with pc := pc`;
-val upd_reg_def  = Define `upd_reg r v s = s with regs := (r =+ v) s.regs`;
-val upd_mem_def  = Define `upd_mem a b s = s with mem := (a =+ b) s.mem`;
-val read_reg_def  = Define `read_reg r s = s.regs r`;
-val read_mem_def  = Define `read_mem a s = s.mem a`;
+val upd_pc_def   = Define `upd_pc pc s = s with pc := pc`
+val upd_reg_def  = Define `upd_reg r v s = s with regs := (r =+ v) s.regs`
+val upd_mem_def  = Define `upd_mem a b s = s with mem := (a =+ b) s.mem`
+val read_reg_def = Define `read_reg r s = s.regs r`
+val read_mem_def = Define `read_mem a s = s.mem a`
 
-val assert_def = Define `
-  assert b s = s with failed := (~b \/ s.failed)`;
+val assert_def = Define `assert b s = s with failed := (~b \/ s.failed)`
 
 val reg_imm_def = Define `
   (reg_imm (Reg r) s = read_reg r s) /\
-  (reg_imm (Imm w) s = w)`;
+  (reg_imm (Imm w) s = w)`
 
 val binop_upd_def = Define `
-  (binop_upd r Add w1 w2 =
-     upd_reg r (w1 + w2)) /\
-  (binop_upd r Sub w1 w2 =
-     upd_reg r (w1 - w2)) /\
-  (binop_upd r And w1 w2 =
-     upd_reg r (word_and w1 w2)) /\
-  (binop_upd r Or w1 w2 =
-     upd_reg r (word_or w1 w2)) /\
-  (binop_upd r Xor w1 w2 =
-     upd_reg r (word_xor w1 w2))`
+  (binop_upd r Add w1 w2 = upd_reg r (w1 + w2)) /\
+  (binop_upd r Sub w1 w2 = upd_reg r (w1 - w2)) /\
+  (binop_upd r And w1 w2 = upd_reg r (word_and w1 w2)) /\
+  (binop_upd r Or w1 w2  = upd_reg r (word_or w1 w2)) /\
+  (binop_upd r Xor w1 w2 = upd_reg r (word_xor w1 w2))`
 
 val word_cmp_def = Define `
   (word_cmp Equal w1 w2 = (w1 = w2)) /\
-  (word_cmp Less w1 w2 = (w1 < w2)) /\
+  (word_cmp Less w1 w2  = (w1 < w2)) /\
   (word_cmp Lower w1 w2 = (w1 <+ w2)) /\
-  (word_cmp Test w1 w2 = (w1 && w2 = 0w))`;
+  (word_cmp Test w1 w2  = (w1 && w2 = 0w))`
 
 val word_shift_def = Define `
   (word_shift Lsl w n = w << n) /\
   (word_shift Lsr w n = w >>> n) /\
-  (word_shift Asr w n = w >> n)`;
+  (word_shift Asr w n = w >> n)`
 
 val arith_upd_def = Define `
   (arith_upd (Binop b r1 r2 (ri:'a reg_imm)) s =
@@ -236,35 +234,34 @@ val arith_upd_def = Define `
        (upd_reg r1 (word_shift l (read_reg r2 s) n) s))`
 
 val addr_def = Define `
-  addr (Addr r offset) s =
-    (read_reg r s + offset)`
+  addr (Addr r offset) s = read_reg r s + offset`
 
 val read_mem_word_def = Define `
   (read_mem_word a 0 s = (0w:'a word,s)) /\
   (read_mem_word a (SUC n) s =
-     let (w,s1) = read_mem_word (a+1w) n s in
+     let (w,s1) = read_mem_word (a + 1w) n s in
        (word_or (w << 8) (w2w (read_mem a s1)),
-          assert (a IN s1.mem_domain) s1))`;
+          assert (a IN s1.mem_domain) s1))`
 
 val mem_load_def = Define `
   mem_load n r a s =
     let a = addr a s in
     let (w,s) = read_mem_word a n s in
     let s = upd_reg r w s in
-      assert (a && n2w (n-1) = 0w) s`
+      assert (a && n2w (n - 1) = 0w) s`
 
 val write_mem_word_def = Define `
   (write_mem_word a 0 w s = s) /\
   (write_mem_word a (SUC n) w s =
-     let s1 = write_mem_word (a+1w) n (w >>> 8) s in
-       assert (a IN s1.mem_domain) (upd_mem a (w2w w) s1))`;
+     let s1 = write_mem_word (a + 1w) n (w >>> 8) s in
+       assert (a IN s1.mem_domain) (upd_mem a (w2w w) s1))`
 
 val mem_store_def = Define `
   mem_store n r a s =
     let a = addr a s in
     let w = read_reg r s in
     let s = write_mem_word a n w s in
-      assert (a && n2w (n-1) = 0w) s`
+      assert (a && n2w (n - 1) = 0w) s`
 
 val mem_op_upd_def = Define `
   (mem_op Load r a = mem_load (dimindex (:'a) DIV 8) r a) /\
@@ -272,16 +269,16 @@ val mem_op_upd_def = Define `
   (mem_op Load8 r a = mem_load 1 r a) /\
   (mem_op Store8 r a = mem_store 1 r a) /\
   (mem_op Load32 r (a:'a addr) = mem_load 4 r a) /\
-  (mem_op Store32 r (a:'a addr) = mem_store 4 r a)`;
+  (mem_op Store32 r (a:'a addr) = mem_store 4 r a)`
 
 val inst_def = Define `
   (inst (Const r imm) s = upd_reg r imm s) /\
   (inst (Arith x) s = arith_upd x s) /\
-  (inst (Mem m r a) s = mem_op m r a s)`;
+  (inst (Mem m r a) s = mem_op m r a s)`
 
 val inst_opt_def = Define `
   (inst_opt NONE s = s) /\
-  (inst_opt (SOME i) s = inst i s)`;
+  (inst_opt (SOME i) s = inst i s)`
 
 val jump_to_offset_def = Define `
   jump_to_offset w s = upd_pc (s.pc + w) s`
@@ -289,8 +286,7 @@ val jump_to_offset_def = Define `
 val asm_def = Define `
   (asm Skip pc s = upd_pc pc s) /\
   (asm (Inst i) pc s = upd_pc pc (inst i s)) /\
-  (asm (Jump l i) pc s =
-     inst_opt i (jump_to_offset l s)) /\
+  (asm (Jump l i) pc s = inst_opt i (jump_to_offset l s)) /\
   (asm (JumpCmp cmp r ri l i) pc s =
      if word_cmp cmp (read_reg r s) (reg_imm ri s)
      then inst_opt i (jump_to_offset l s)
@@ -300,13 +296,13 @@ val asm_def = Define `
   (asm (Loc r l) pc s = upd_pc pc (upd_reg r (s.pc + l) s))`
 
 val bytes_in_memory_def = Define `
-  (bytes_in_memory a [] m dm <=> T) /\
-  (bytes_in_memory a ((x:word8)::xs) m dm <=>
-     (m a = x) /\ a IN dm /\ bytes_in_memory (a+1w) xs m dm)`;
+  (bytes_in_memory a [] m dm = T) /\
+  (bytes_in_memory a ((x:word8)::xs) m dm =
+     (m a = x) /\ a IN dm /\ bytes_in_memory (a + 1w) xs m dm)`
 
 val asm_step_def = Define `
   asm_step enc c s1 s2 =
-    ?i. ~(s2.failed) /\ asm_ok i c /\
+    ?i. ~s2.failed /\ asm_ok i c /\
         bytes_in_memory s1.pc (enc i) s1.mem s1.mem_domain /\
         (asm i (s1.pc + n2w (LENGTH (enc i))) s1 = s2)`
 
@@ -317,24 +313,23 @@ val enc_deterministic_def = Define `
     !i j s1.
       asm_ok i c /\ asm_ok j c /\ isPREFIX (enc i) (enc j) ==>
         (asm i (s1.pc + n2w (LENGTH (enc i))) s1 =
-         asm j (s1.pc + n2w (LENGTH (enc j))) s1)`;
+         asm j (s1.pc + n2w (LENGTH (enc j))) s1)`
 
 val bytes_in_memory_IMP = prove(
   ``!xs ys a m dm.
-      bytes_in_memory a xs m dm /\
-      bytes_in_memory a ys m dm ==>
+      bytes_in_memory a xs m dm /\ bytes_in_memory a ys m dm ==>
       isPREFIX xs ys \/ isPREFIX ys xs``,
-  Induct THEN Cases_on `ys` THEN SRW_TAC [] []
-  THEN METIS_TAC [bytes_in_memory_def]);
+  Induct
+  THEN Cases_on `ys`
+  THEN SRW_TAC [] []
+  THEN METIS_TAC [bytes_in_memory_def])
 
 val asm_deterministic = store_thm("asm_deterministic",
   ``enc_deterministic enc config ==>
     !s1 s2 s3.
-      asm_step enc config s1 s2 /\
-      asm_step enc config s1 s3 ==>
-        (s2 = s3)``,
+      asm_step enc config s1 s2 /\ asm_step enc config s1 s3 ==> (s2 = s3)``,
   SRW_TAC [] [asm_step_def]
-  THEN METIS_TAC [enc_deterministic_def,bytes_in_memory_IMP]);
+  THEN METIS_TAC [enc_deterministic_def, bytes_in_memory_IMP])
 
 (* -- well-formedness of encoding -- *)
 
@@ -343,7 +338,7 @@ val enc_ok_def = Define `
     (* code alignment *)
     1 <= c.code_alignment /\
     ((c.code_alignment = 1) ==> ODD (LENGTH (enc Skip))) /\
-    (!w. (LENGTH (enc w)) MOD c.code_alignment = 0) /\
+    (!w. LENGTH (enc w) MOD c.code_alignment = 0) /\
     (* label instantiation does not affect length of code *)
     (!w i. LENGTH (enc (Jump w i)) = LENGTH (enc (Jump 0w i))) /\
     (!c r ri w i. LENGTH (enc (JumpCmp c r ri w i)) =
@@ -351,16 +346,15 @@ val enc_ok_def = Define `
     (!w r. LENGTH (enc (Call w r)) = LENGTH (enc (Call 0w r))) /\
     (!w r. LENGTH (enc (Loc r w)) = LENGTH (enc (Loc r 0w))) /\
     (* no overlap between instructions with different behaviour *)
-    enc_deterministic enc c`;
+    enc_deterministic enc c`
 
 (* -- correctness property to be proved for each backend -- *)
 
 val backend_correct_def = Define `
-  backend_correct enc (config:'a asm_config) (next:'b->'b) assert =
+  backend_correct enc (config:'a asm_config) (next:'b -> 'b) R =
     enc_ok enc config /\
     !s1 s2.
       asm_step enc config s1 s2 ==>
-      !state. assert s1 state ==>
-              ?n. assert s2 (FUNPOW next (n+1) state)`;
+      !state. R s1 state ==> ?n. R s2 (FUNPOW next (n + 1) state)`
 
-val _ = export_theory();
+val () = export_theory ()
